coq/circuits: Optimize redundant & and |; apply optimizers iteratively

ocaml/cuttlebone/cuttlebone.ml
@@ -360,7 +360,7 @@ module Compilation = struct
     (* let equivb _ c1 c2 = c1 == c2 in *)
     let equivb = extr_circuit_incomplete_equivb in
     let cR, cSigma = lower_R _R, lower_Sigma _Sigma in
-    lco_opt_compose cR cSigma (opt_constprop cR cSigma) (opt_muxelim cR cSigma equivb)
+    (lco_all_iterated cR cSigma equivb 10).lco_fn
 
   let compile (cu: 'f compile_unit) : (reg_signature -> compiled_circuit) =
     let finiteType = Util.finiteType_of_list cu.c_registers in
